Add test for Set.OrdPair

rocq/ZF/Meta/Decl/Set/OrdPair.v
@@ -1,6 +1,7 @@
 Require Import Coq.Lists.List.
 Require Import Coq.Strings.String.
 
+Require Import ZF.Meta.DeclP.
 Require Import ZF.Meta.DeclT.
 Require Import ZF.Meta.Env.
 Require Import ZF.Meta.Syntax.
@@ -9,17 +10,94 @@ Require Import ZF.Meta.Ty.
 Import ListNotations.
 Open Scope string_scope.
 
+Require Import ZF.Meta.Decl.Set.Pair.
+Require Import ZF.Meta.Decl.Set.Single.
+
 (* ordPair a b : U.                                                             *)
 Definition ordPair : DeclT :=
   {| paraT := [TySet; TySet]
   ;  resT  := TySet
-  ;  bodyT := HoleT TySet
+  ;  bodyT :=
+      IdentT (Name.local "pair")
+        (args [IdentT (Name.local "single") (args [Var 1]);
+         IdentT (Name.local "pair") (args [Var 1; Var 0])])
   |}.
 
-Definition imports : Env := Env.empty.
+(* forall a b x, x :< ordPair a b <-> x = single a \/ x = pair a b.             *)
+Definition Charac : DeclP :=
+  let concl :=
+    All
+      (All
+        (All
+          (Iff
+            (Elem (Var 0)
+              (IdentT (Name.local "ordPair") (args [Var 2; Var 1])))
+            (Or
+              (Equal (Var 0)
+                (IdentT (Name.local "single") (args [Var 2])))
+              (Equal (Var 0)
+                (IdentT (Name.local "pair") (args [Var 2; Var 1])))))))
+  in
+    {| paraP  := []
+    ;  conclP := concl
+    ;  bodyP  := HoleP concl
+    |}.
 
-Definition exports : Env := Env.fromListT
-  [ (Name.local "ordPair", ordPair)
+(* forall a b c, single a = pair b c -> a = b /\ a = c.                         *)
+Definition ABC : DeclP :=
+  let concl :=
+    All
+      (All
+        (All
+          (Imp
+            (Equal
+              (IdentT (Name.local "single") (args [Var 2]))
+              (IdentT (Name.local "pair") (args [Var 1; Var 0])))
+            (And
+              (Equal (Var 2) (Var 1))
+              (Equal (Var 2) (Var 0))))))
+  in
+    {| paraP  := []
+    ;  conclP := concl
+    ;  bodyP  := HoleP concl
+    |}.
+
+(* forall a b c d, ordPair a b = ordPair c d -> a = c /\ b = d.                 *)
+Definition Equal : DeclP :=
+  let concl :=
+    All
+      (All
+        (All
+          (All
+            (Imp
+              (Equal
+                (IdentT (Name.local "ordPair") (args [Var 3; Var 2]))
+                (IdentT (Name.local "ordPair") (args [Var 1; Var 0])))
+              (And
+                (Equal (Var 3) (Var 1))
+                (Equal (Var 2) (Var 0)))))))
+  in
+    {| paraP  := []
+    ;  conclP := concl
+    ;  bodyP  := HoleP concl
+    |}.
+
+(* Environment.                                                                 *)
+
+Definition imports : Env := Env.unions
+  [ Env.unqualify Pair.exports
+  ; Env.unqualify Single.exports
+  ].
+
+Definition exports : Env := Env.unions
+  [ Env.fromListT
+      [ (Name.local "ordPair", ordPair)
+      ]
+  ; Env.fromListP
+      [ (Name.local "Charac", Charac)
+      ; (Name.local "ABC"   , ABC)
+      ; (Name.local "Equal" , Equal)
+      ]
   ].
 
 Definition env : Env := Env.union imports exports.
