rocq/ZF/Set/OrdPair.v
@@ -12,14 +12,14 @@ Definition ordPair (a b:U) : U := :{ :{a}: , :{a,b}: }:.
 Notation ":( a , b ):" := (ordPair a b)
   (at level 1, no associativity) : ZF_Set_OrdPair_scope.
 
-Lemma Charac : forall (a b:U),
+Proposition Charac : forall (a b:U),
   forall x, x :< :(a,b): <-> x = :{a}: \/ x = :{a,b}:.
 Proof.
   intros a b. apply Pair.Charac.
 Qed.
 
 (* If the singleton {a} equals the pair {b,c}, then a = b and a = c.            *)
-Lemma ABC : forall a b c, :{a}: = :{b,c}: -> a = b /\ a = c.
+Local Proposition ABC : forall a b c, :{a}: = :{b,c}: -> a = b /\ a = c.
 Proof.
   intros a b c Habc. split.
   - symmetry. apply Single.Charac. rewrite Habc. apply Pair.IsInL.
